$\textrm{Para y = 1}$

${2y} ^ {2} -3y=2×1-3×1=-1  $\
$ 4y-1=4×1-1=3 $\
$  {6y} ^ {2} +1=6×1+1=7$

$\textrm{Para y = }\dfrac{3}{8}$

${2y} ^ {2} -3y=2× { (\dfrac{3} {8} )} ^ {2} -3× \dfrac{3} {8} =- \dfrac{27} {32}$

$ 4y-1=4× \dfrac{3} {8} -1= \dfrac{3} {2} - \dfrac{2} {2} = \dfrac{1}  {2}  $~

$  {6y} ^ {2} +1=6× { (\dfrac{3} {8} )} ^ {2} +1=6× \dfrac{9} {64} + \dfrac{64} {64} = \dfrac{54} {64} +\dfrac {64} {64} = \dfrac{59} {32}$

$\textrm{Logo, os termos são -1, 3 e 7 ou .} - \dfrac{27} {32} ,  \dfrac{1} {2}  e  \dfrac{59} {32}$